Implement and verify SETATTR

nfsd/ops.go
@@ -154,31 +154,11 @@ func (nfs *Nfs) NFSPROC3_SETATTR(args nfstypes.SETATTR3args) nfstypes.SETATTR3re
 		reply.Status = nfstypes.NFS3ERR_NOTSUPP
 		return reply
 	}
-	if args.New_attributes.Mode.Set_it {
-		util.DPrintf(1, "NFS SetAttr ignore mode %v\n", args)
-	}
-	if args.New_attributes.Uid.Set_it {
-		util.DPrintf(1, "NFS SetAttr uid not supported %v\n", args)
-	}
-	if args.New_attributes.Gid.Set_it {
-		util.DPrintf(1, "NFS SetAttr gid not supported %v\n", args)
-	}
-	if args.New_attributes.Atime.Set_it != nfstypes.DONT_CHANGE {
-		util.DPrintf(1, "NFS SetAttr atime not supported")
-	}
-	if args.New_attributes.Mtime.Set_it != nfstypes.DONT_CHANGE {
-		util.DPrintf(1, "NFS SetAttr mtime not supported")
-	}
-	// we don't support any other attributes
-	if !args.New_attributes.Size.Set_it {
-		reply.Status = nfstypes.NFS3_OK
-		return reply
-	}
 	inum := fh2ino(args.Object)
-	size := uint64(args.New_attributes.Size.Size)
+	sattr := encodeSattr3(args.New_attributes)
 
 	_, status := nfs.runTxn(func(txn Txn) Result {
-		return nfs.filesys.SETATTRsize(txn, inum, size)
+		return nfs.filesys.SETATTR(txn, inum, sattr)
 	})
 	reply.Status = status
 
